---
title: "1.1. Language and Logic"
date: "2023-08-15"
tags:
---

1.1.1. Basic connectives

## Logic

### And

|P|Q|P $\textasciicircum$ Q|
|---|---|---|
|T|T|T|
|T|F|F|
|F|T|F|
|F|F|F|


### Table

|P|Q|¬P|¬Q|P∧Q|¬(P∧Q)|¬P∧¬Q|¬P∨¬Q|
|---|---|---|---|---|---|---|---|
|T|T|F|F|T|F|F|F| 
|T|F|F|T|F|T|F|T| 
|F|T|T|F|F|T|F|T| 
|F|F|T|T|F|T|T|T|

### Distributing ¬

#### DeMorgan's Laws
![[notes/Mathematics/TTOMR/DeMorgan's Laws|DeMorgan's Laws]]

### Implication

|P|Q|P⇒Q|
|---|---|---|
|T|T|T|
|T|F|F|
|F|T|T|
|F|F|T|

In the statement P ⇒ Q, P is called the hypothesis, or antecedent, and Q is called the conclusion or consequent.

The logical equivalent to P⇒Q is ¬P ∨ Q

### Biconditional

interpret the ⇐ of P ⇔ Q as *if* and the ⇒ as *only if*

### Proposition 1.1.11
1. P ⇒ Q is logically equivalent to (¬P ) ∨ Q
2. ¬(P ⇒ Q) is logically equivalent to P ∧ (¬Q)
3. P ⇔ Q is true exactly when P and Q have the same truth value.

### Contrapositive

The contrapositive of P ⇒ Q is ¬Q ⇒ ¬P
The contrapositive is logically equivalent to the original

P ⇒ Q and its contrapositive (¬Q) ⇒ (¬P) are logically equivalent

![[notes/Mathematics/TTOMR/Proposition 1.1.15|Proposition 1.1.15]]

## Quantifiers

Let $\mathbb{U}$ be the universe under consideration and P(x) be a predicate whose only free variable is x

Notation: 
“for all x, P(x)”                                        notation: (∀x)P(x)
“there exists x such that P(x)”              notation: (∃x)P(x)

$\forall$ is the universal quantifier and ($\forall$x)P(x) is true exactly when each element a in Universe $\mathbb{U}$ has the property that P(a) true

$\exists$ is the existential quantifier and ($\exists$)P(x) is true exactly when the Universe $\mathbb{U}$ contains at least one element a such that P(a) true

The universe can be explicit using notation ($\forall$x $\in \mathbb{U}$)P(x)

### Table 1.10. Number universes

natural numbers $\mathbb{N}$: $\mathbb{N}$ = { 1, 2, 3, ... }
integers $\mathbb{Z}$: $\mathbb{Z}$ = { ..., -3, -2, -1, 0, 1, 2, 3, ... }
rational numbers $\mathbb{Q}$: x $\in \mathbb{Q}$ if there exists a, b $\in \mathbb{Z}$, b $\neq$ 0 such that x = $\frac{a}{b}$
real numbers $\mathbb{R}$: informally, x $\in \mathbb{R}$ if x has a decimal expansion

The set of positive integers may be represented as $\mathbb{Z} ^{+}$

### Quantifier Negation

### Proposition 1.1.18
1. ¬(∀x)P (x) is logically equivalent to (∃x)(¬P (x)); i.e., ¬(∀x ∈ U )P (x) is logically equivalent to (∃x ∈ U)(¬P(x))
2. ¬(∃x)P (x) is logically equivalent to (∀x)(¬P (x)); i.e., ¬(∃x ∈ U )P (x) is logically equivalent to (∀x ∈ U)(¬P(x))

Beware of implied quantifiers hidden in language

# Exercises 1.1
1. Let P, Q, and R be statements. Determine whether or not the two expressions in each pair are logically equivalent. In each case, demonstrate that your answer is correct.
	1. a) (P ^ Q) ^ R and P ^ (Q ^ R)
		1. In both cases, all P, Q, R must be true for each value to be true and all other cases are false $\therefore$ truth tables and logic are equivalent
	2. b) (P v Q) v R and P v (Q v R)
		1. In both cases, if any P, Q, R is true, then each value is true
	3. c) (P ^ Q) v R and P ^ (Q v R)
		1. (P ^ Q) v R => (R v P) ^ (R ^ Q)
		2. P ^ (Q v R) => (P ^ Q) v (P ^ R)
		3. (P ^ Q) v (P ^ R) => (P ^ Q) v (P ^ R)
		4. Logically equivalent
	4. d) (P v Q) ^ R => P v (Q ^ R)
		1. (P ^ R) v (Q ^ R) => (P v Q) ^ (P v R)
		2. Not logically equivalent, left requires R to be true whereas right does not
2. Let P, Q, and R be statements. Show that the following statements are logically equivalent
	1. a) $\neg$($\neg$P) => P
	2. b) (P v Q) ^ R => (P ^ R) v (Q ^ R)
		1. (P ^ R) v (Q ^ R) => (P ^ R) v (Q ^ R)
	3. c) (P ^ Q) v R => (P v R) ^ (Q v R)
		1. (P v R) ^ (Q v R) => (P v R) ^ (Q v R)
	4. d) $\neg$(P v Q) => ($\neg$P) ^ ($\neg$Q)
		1. $\neg$(P v Q) => $\neg$P $\neg$v $\neg$Q => ($\neg$P) ^ ($\neg$Q)
	5. e) (P => Q) => ($\neg$P) v Q
		1. | P | Q | P => Q | ($\neg$P) v Q |
			|---|---|---|---|
			|T | T | T | T |
			|F | T | T | T |
			|T | F | F | F |
			|F | F | T | T |
	6. f) \[$\neg$(P => Q)] => (P ^ ($\neg$Q))
		1. (P => Q) => (($\neg$P) v Q)
		2. $\neg$(P => Q) => $\neg$(($\neg$P) v Q)
		3. $\neg$(($\neg$P) v Q) => (P ^ ($\neg$Q))
		4. $\therefore$ \[$\neg$(P => Q)] =>(P ^ ($\neg$Q))
3. Let, P, Q, and R be statements. Determine whether or not the two expressions in each pair are logically equivalent. In each case, demonstrate that your answer is correct.
	1. a) (P => Q) => R and P => (Q => R)
		1. Left: \[(P => Q) => R] => \[$\neg$(P => Q) v R] => \[(P ^ ($\neg$Q)) v R] => \[(P v R) ^ ($\neg$Q v R)]
		2. Right: \[P => (Q => R)] => \[($\neg$P v (Q => R))] => \[$\neg$P v ($\neg$Q v R)] => \[$\neg$P v $\neg$Q v R]
		3. #review
	2. b) (P v Q) => R and (P => R) v (Q => R)

[[notes/Mathematics/TTOMR/1.2 Proof|1.2 Proof]]