---
title: "1.2 Proof"
date: "2023-08-15"
tags:
---

[[notes/Mathematics/TTOMR/1.1. Language and Logic|1.1. Language and Logic]]

1.2.1. Logical Arguments

Informally, a proof is a logical argument that establishes the truth of a mathematical statement

For example,
	(P => Q) If f is differentiable at a, then f is continuous at a
	(P) f is differentiable at a
	$\therefore$ from P and P => Q, deduce Q

Modus ponens: "rule of deduction"

> If we wish to prove a mathematical statement, then we must first determine the logical form of that statement

1.2.2 Direct proofs, and introduction

> To prove a statement of the form P => Q is true (directly)
> - We begin with "Assume P is true"
> - We must then demonstrate that Q is true

> To prove a statement of the form ($\forall$x)P(x) is true (directly)
> - We begin with "Let x b e an arbitrary (but now *fixed*), element of the universe"
> - We must then demonstrate that P(x) is true

> To prove a statement of the form ($\exists$x)P(x) is true (directly)
> - We must find an element a in the universe that that P(a) is true
> - In other words, we must explicitly say what a is and demonstrate that P(a) is true

![[notes/Mathematics/TTOMR/Definition 1.2.1.|Definition 1.2.1.]]

> **Special status of definitions.** *Mathematical definitions are always* **if and only if** *statements.*

We use a "Given-Goal" diagram to identify what is given and what is out goal. 

| Given | Goal | 
| --- | --- |
| $m, n$ arbitrary integers | if $m$ is even and $n$ is odd, then $m + n$ is odd

Right away, the logical structure of the goal, an implication, tells us what to do next

> The Goal dictates the form of the proof

Based on previous table,

| Given | Goal | 
| --- | --- |
| $m, n$ arbitrary integers | |
| $m$ is even | |
| $n$ is odd | $m + n$ is odd |


Given that $m$ is even, this means that
$$
there \text{ } exists \text{ an integer } k \text{ such that } m = 2k
$$
Since such an integer $exists$, we we'll $fix$ one so that we can work with it; i.e., we can
$$
\text{fix } i \in \mathbb{Z} \text{ such that } m=2i
$$
Similarly, since we know
$$
n \text{ is odd},
$$
we can
$$
\text{fix } j \in \mathbb{Z} \text{ such that } n=2j+1
$$
Since we both want information about the integer $m + n$, it makes sense to investigate this quantity. Note that
$$
m + n = 2i + (2j + 1) = (2i + 2j) + 1 = 2(i + j) + 1
$$
Since $i + j$ is an integer, we've found the integer $a$ we are seeking

\[this is formally written in Proposition 1.2.2 on page 35/233]

> If we *know* ($\exists$x)P(x), where P(x) is some predicate involving the free variable $x$, then we should *fix a particular x* such that P(x) holds, as long as we take care *not* to use a variable whose meaning in the current proof is already fixed

![[notes/Mathematics/TTOMR/Prove Something is a Widget|Prove Something is a Widget]]

Basic Properties of Integers
![[notes/Mathematics/TTOMR/Basic Properties of Integers 1.2.3|Basic Properties of Integers 1.2.3]]

# Exercises 1.2

1. Let $n$ be an integer
	1. a) Prove that if $n$ is even, then $n^{2}$ is even
		1. $n = 2i$ for arbitrary $i\in \mathbb{Z}$
		2. $n^{2} = (2i)^{2} = 4i^{2} = 2(2i^{2})$ which is even by definition
	2. b) Prove that if $n$ is odd, then $n^{2}$ is odd
		1. $n = 2i + 1$ for arbitrary $i \in \mathbb{Z}$
		2. $n^{2} = (2i+1)^{2} = 4i^{2} + 4i + 1 = 2(2i^{2} + 2i) + 1$ which is odd by definition
2. Let $m$ and $n$ be integers
	1. a) Prove that if $m$ and $n$ are even, then $m+n$ is even
		1. $m = 2i, n = 2j$ for arbitrary $i,j\in \mathbb{Z}$
		2. $m+n=2i+2j=2(i+j)$ which is even by definition
	2. b) Prove that if $m$ and $n$ are odd, then $m+n$ is odd
		1. $m=2i+1,n=2j+1$ for arbitrary $i,j \in \mathbb{Z}$
		2. $m+n=2i+1+2j+1=2i+2j+2=2(i+j+1)$ which is even by definition
3. 
	1. a) Prove that for all $m \in \mathbb{Z}$, if $m$ is even, then $mn$ is even
		1. $m=2i$ for arbitrary $i,n \in \mathbb{Z}$
		2. $mn=2in$ which is even by definition
	3. b) Prove that for all $m$, $n \in \mathbb{Z}$, if $m$ and $n$ are odd, then $mn$ is odd
		1. $m =2i + 1, n=2j+1$ for arbitrary $i,j \in \mathbb{Z}$
		2. $mn = (2i+1)(2j+1) = 4ij + 2i + 2j + 1 = 2(2ij + i + j) + 1$ which is odd by definition
4. Use the definition to prove that for all $n \in \mathbb{N}, 4n+7$ is odd
	1. $4n+7=2(2n+3)+1$, $(2n+3) \in \mathbb{Z}$, $\therefore$ $4n + 7$ is odd by definition