---
title: "2.1.5. Uniqueness proofs"
date: "2023-08-15"
tags:
---

Sometimes we find that not only do we wish to prove that an object exists, hut also we wish to prove that the object that exists is *unique*. i.e., that there is exactly one such object. We can express this in our mathematical language in one of two ways. Suppose that $P(x)$ is a predicate with free variable $x$, and think of $P(x)$ as expressing "$x$ satisfies property $P$". The statement
$$
\text{there exists a unique } x \text{ such that } P(x)
$$
denotes
$$
(\exists x)[P(x) \wedge (\forall y)[P(y) \implies x=y]]
\tag{2.6}
$$
or
$$
(\exists x)P(x) \wedge (\forall y)(\forall z)[(P(y) \wedge P(z)) \implies y =z]
\tag{2.7}
$$
Remember that $\wedge$ denotes the logical connection "and".

Statement (2.6) states that
1) an object $x$ satisfying property $P$ exists and, furthermore,
2) if $y$ is an arbitrary object satisfying property $P$, then $u$ myst be the same object as this $x$
Statement (2.7) states that
1) an object $x$ satisfying property $P$ exists, and
2) if $y$ and $z$ are arbitrary objects both satisfying property $P$, then $y$ and $z$ are equal.

Both statement (2.6) and statement (2.7) can be represented by the notation
$$
(\exists!x)P(x)
$$
Regardless of whether one thinks of $(\exists!x)P(x)$ in terms of statement (2.6) or statement (2.7), note that a proof of $(\exists!x)P(x)$ always has two parts: a proof of *existence* and a proof of *uniqueness*.

![[notes/Mathematics/TTOMR/Example 2.1.13.|Example 2.1.13.]]

The point of this example was to illustrate a standard uniqueness proof, and it is necessary to prove statements of this sort in an abstract algebra course. We'll see more uniqueness statements later in this textbook.