---
title: "2.2.2. Proving the contrapositive"
date: "2023-08-15"
tags:
---

To motivate our second method of indirect proof, we will show that
$$
\boxed{\text{for all } n\in\mathbb{Z} \text{, if } n^2 \text{ if odd, then } n \text{ is odd}}
$$
It's easy to see why we should try to use an indirect proof.

| Given | Goal |
| --- | --- |
| $n\in\mathbb{Z}$ arbitrary | |
| $n^2$ is odd | $n$ is odd |

If we assume that $n\in\mathbb{Z}$ with $n^2$ odd, then by Definition 1.2.1, we know that we may fix $k\in\mathbb{Z}$ such that $n^2=2k+1$. However, this does not give us any information about $n$. We could use a proof by contradiction here (try it yourself), but we will instead take advantage of what we know about implications.

Recall from [[notes/Mathematics/TTOMR/Proposition 1.1.15|Proposition 1.1.15]] that an implication $P\implies Q$ is logically equivalent to its contrapositive $\neg Q \implies \neg P$.
$$
\boxed{\text{Thus, to prove } P\implies Q,\text{ we may choose instead to prove } \neg Q\implies \neg P}
$$
The contrapositive of
$$
n^2 \text{ is odd}\implies n \text{ is odd}
$$
is
$$
n \text{ is even } \implies n^2 \text{ is even}
$$
We certainly know how to prove this (see Exercise 1.2.1a),  and proving this statement servers as a proof of our original statement, since the two statements are logically equivalent. For practice, however, rather than simply quoting Exercise 1.2.1a, we'll provide all details in this proof.

| Given | Goal |
| --- | --- |
| $n\in\mathbb{Z}$ arbitrary | |
| $n$ is even | $n^2$ is even |

![[notes/Mathematics/TTOMR/Proposition 2.2.3.|Proposition 2.2.3.]]

![[notes/Mathematics/TTOMR/Proposition 2.2.4.|Proposition 2.2.4.]]

# Proving or statements
In this section we consider one useful method of proving a statement which is disjunction. Consider the following proposition.

![[notes/Mathematics/TTOMR/Proposition 2.2.5.|Proposition 2.2.5.]]

As usual, we begin with a Given-Goal diagram.

| Given | Goal |
| --- | --- |
| $a,b\in\mathbb{R}$ arbitrary | |
| $b\geq 0$ | |
| $a^2\geq b^2$ | $a\geq \sqrt{ b }$ or $a\leq-\sqrt{ b }$ |

We could try a proof by contradiction here. Instead, we will once again take advantage of logic. Recall from Proposition 1.1.11 and Exercise 1.1.2a that a statement of the form $P \lor Q$ is logically equivalent to the statement $\neg P \implies Q$. Also note that $P \lor Q$ is logically equivalent to $Q \lor P$, which is logically equivalent to the statement $\neg Q \implies P$.
$$
\boxed{\text{Thus, to prove } P \lor Q, \text{ we may assume } \neg P \text{ and prove } Q, \text{ or we may assume } \neg Q \text{ and prove } P.}
$$
Since we are not proving the statement in its original form, we view this method of proving $P \lor Q$ as an indirect proof. We an also think of this as a proof by cases, where one of the cases is automatic. for example, if $P$ is true, then $P \lor Q$ is automatically true; thus, we need only consider the case when $P$ is false; i.e., when $\neg P$ is true. The analogous approach with the roles of $P$ and $Q$ interchanged is also permitted.

Note that in this case either of the statements $a\geq \sqrt{ b }$ or $q\leq-\sqrt{ b }$ can be $P$. In general, however, your choice of $P$ and $Q$ will depend on the statements themselves and whatever is easier to work with. The new Given-Goal diagram follows.

| Given | Goal |
| --- | --- |
| $a,b\in\mathbb{R}$ | |
| $b\geq 0$ | |
| $a^2\geq b$ | |
| $a\ngeq b$ (i.e., $a<\sqrt{ b }$) | $a\leq -\sqrt{ b }$ |

To deal with these inequalities, it often helps to express them by moving all the terms to one side. Thus we have $a^2-b^2\geq 0$, so we can manipulate by factoring (remember that $b\in\mathbb{R}$ with $b\geq 0$):
$$
(a-\sqrt{ b })(a+\sqrt{ b }) \geq 0
$$
We are also given that $a-\sqrt{ b }<0$, so it's now easy to see how this proof should go

![[notes/Mathematics/TTOMR/Proof of Proposition 2.2.5.|Proof of Proposition 2.2.5.]]