---
title: "3.1 Principle of Mathematical Induction"
date: "2023-08-15"
tags:
---

# Previous
[[notes/Mathematics/TTOMR/2.4. Proofs of statements involving mixed quantifiers|2.4. Proofs of statements involving mixed quantifiers]]
# Introduction
Thus far we have been proving results about the integers using only the assumptions in the [[notes/Mathematics/TTOMR/Basic Properties of Integers 1.2.3|Basic Properties of Integers 1.2.3]]. Up to now, any direct proof of a statement of the form $(\forall n\in\mathbb{Z}^{+})P(n)$ has begun with the assumption "Let $n\in\mathbb{Z}^{+}$ be arbitrary." We consider now a new proof technique, called *proof by induction*, for proving a statement about *all* positive integers. The statement of the *Principle of Mathematical Induction* is logically complicated, so we have typeset in **bold** the words showing the logical structure of this statement. 
# PMI
![[notes/Mathematics/TTOMR/Theorem 3.1.1. (Principle of Mathematical Induction (PMI))|Theorem 3.1.1. (Principle of Mathematical Induction (PMI))]]
# Notation
![[notes/Mathematics/TTOMR/Notation 3.1.2.|Notation 3.1.2.]]
# Example
For our first example of a proof using PMI, we will prove a summation formula you may have seen before, perhaps when discussing Riemann sums in calculus. We will prove by induction that for all $n\in\mathbb{Z}^{+}$,
$$
\sum_{k=1}^{n}k=\frac{n(n+1)}{2}
$$
$$
\text{i.e., } 1+2+\dots+n=\frac{n(n+1)}{2}
$$
For example, when $n=4$, note that 
$$
\sum_{k=1}^{4}k=1+2+3+4=10 \quad \text{ and } \quad \frac{n(n+1)}{2}=\frac{4(5)}{2}=10
$$
so the statement is true when $n=4$. To prove he statement is true for *all* positive integers $n$, however, we will use PMI. In this first example, we will show our scratch work in great detail.

*Scratch work:* Given $n\in\mathbb{Z}^{+}$, we'll let $P(n)$ be the statement
$$
\sum_{k=1}^{n}k=\frac{n(n+1)}{2}
$$
Note that $P(n)$ is a *statement* about $n$; it asserts that $n$ has a particular property. The Principle of Mathematical Induction says that if we can prove tha the *Base Case* (PMI 1) is true and the *Inductive Step* (PMI 2) is true, then we may *conclude* that $(\forall n\in\mathbb{Z}^{+})P(n)$ is true, which is what we want.

**Base Case:** *Show $P(1)$ is true.*
$P(1)$ is the statement
$$
\sum_{k=1}^{1}k=\frac{1(1+1)}{2},
$$
and our task is to prove that $P(1)$ is true. Thus, we must compute both quantities
$$
\sum_{k=1}^{1}k \text{ and } \frac{1(1+1)}{2}
$$
individually, and then we must verify that these quantities are equal. Note that
$$
\sum_{k=1}^{1}k=1
$$
by definition. Also note that
$$
\frac{1(1+1)}{2}=\frac{2}{2}=1
$$
So we see that
$$
\sum_{k=1}^{1}k=\frac{1(1+1)}{2}
$$
i.e., $P(1)$ is true.

**Inductive Step:** Prove statement (PMI 2). Let's begin with a Given-Goal diagram

| Given | Goal |
| --- | --- |
| $m\in\mathbb{Z}^{+}$ arbitrary | |
| $P(m)$ is true | $P(m+1)$ is true |

which we rewrite as

| Given | Goal |
| --- | --- |
| $m\in\mathbb{Z}^{+}$ arbitrary | |
| $\sum_{k=1}^{m}k=\frac{m(m+1)}{2}$  | $\sum_{k=1}^{m+1}k=\frac{(m+1)((m+1)+1)}{2}$ |

We will *use the Given* (called the *Inductive Hypothesis*), which says that
$$
\tag{3.1}
\sum_{k=1}^{m}k=\frac{m(m+1)}{2}
$$
to help us *prove our Goal*, which says that
$$
\sum_{k=1}^{m+1}k=\frac{(m+1)((m+1)+1)}{2}
$$
We may rewrite our Goal as
$$
\sum_{k=1}^{m+1}k=\frac{(m+1)(m+2)}{2}
$$
$$
\boxed{\text{To prove an equality, we must pick one side and attempt to}}
$$
$$
\boxed{\text{manipulate legally until we reach the other side.}}
$$
We'll start with $\sum_{k=1}^{m+1}k$. The key point in the proof is that, since $m\in\mathbb{Z}^{+}$, 
$$
\sum_{k=1}^{m+1}k=1+2+\dots+(m+1)
$$
$$
= (1+2+\dots+m)+(m+1);
$$
i.e.,
$$
\tag{3.2}
\sum_{k=1}^{m+1}k=(\sum_{k=1}^{m}k)+(m+1)
$$
by the associative property of addition. Equation (3.2) shows us clearly where the Inductive Hypothesis (3.1) will be useful; namely, we may replace $\sum_{k=1}^{m}k$ by $\frac{m(m+1)}{2}$. From here, the computation should be routine.

In our formal writeup of this proof by induction, pay close attention to the *format* of our proof, which we'll use in all proofs by induction.

![[notes/Mathematics/TTOMR/Proposition 3.1.3.|Proposition 3.1.3.]]

Note that the idea of proof by induction is the same idea used when making an "inductive" or "recursive" definition. For example, the familiar function $2^n$, where $n\geq 0$ is an integer, is defined by recursion as follows:
$$
2^0=1
$$
and
$$
\text{for all } m\geq 0, \quad 2^{m+1}=2 \cdot 2^m
$$
Note that, just as with a proof by induction, a recursive definition has a *base case* (sometimes more than one) and an *inductive step*, which in a recursive definition is often called the *recursive step*. Not surprisingly, one often uses proof by induction to prove statements about concepts that are defined recursively.

The factorial function $n!$ is also defined by recursion on $n\geq 0$:
$$
0!=1
$$
and
$$
\text{for all } m\geq 0, (m+1)!=(m+1)m!
$$
For example (showing all steps in the recursion),
$$
5! = 5 \cdot 4!
$$
$$
\quad = 5 \cdot 4 \cdot 3!
$$
$$
\quad = 5 \cdot 4 \cdot 3 \cdot 2!
$$
$$
\quad = 5 \cdot 4 \cdot 3 \cdot 2 \cdot 1!
$$
$$
\quad = 5 \cdot 4 \cdot 3 \cdot 2 \cdot 1 \cdot 0!
$$
$$
\quad = 5 \cdot 4 \cdot 3 \cdot 2 \cdot 1, \quad \text{ since $0!=1$; i.e.,}
$$
$$
5! = 120
$$
Notice also that in a recursive definition or proof by induction, the base case need not correspond to $n=1$, as it did in [[notes/Mathematics/TTOMR/Proposition 3.1.3.|Proposition 3.1.3.]], nor to $n=0$, as it did in the recursive definition above. Thus, we can state a more general version of the Principle of Mathematical Induction.

![[notes/Mathematics/TTOMR/Theorem 3.1.4. (Principle of Mathematical Induction (modified))|Theorem 3.1.4. (Principle of Mathematical Induction (modified))]]

# Exercises
![[notes/Mathematics/TTOMR/Exercises 3.1|Exercises 3.1]]
# Next
[[notes/Mathematics/TTOMR/3.2. Strong Induction|3.2. Strong Induction]]